DataflowRewriter/LockedQueue.lean
@@ -54,36 +54,12 @@ instance SpecStateTransition : StateTransition Method SpecState where
 
 infix:60 " ≺ " => @indistinguishable Method
 
-inductive φ' : ImpState → SpecState → Prop where
-  | base :
-    φ' ⟨false, []⟩ ⟨[]⟩
-  | enq : ∀ i (i' : Nat → ImpState) s (s' : Nat → SpecState),
-    (∀ n, i' n = { i with queue := i.queue ++ [n] }) →
-    (∀ n, s' n = { s with queue := s.queue ++ [n] }) →
-    (∀ n, φ' (i' n) (s' n)) →
-    (∀ n, imp_step i [Method.enq n] (i' n)) →
-    (∀ n, spec_step s [Method.enq n] (s' n)) →
-    φ' i s
-  | deq : ∀ i i' s s',
-    φ' i' s' →
-    imp_step i [Method.deq n] i' →
-    spec_step s [Method.deq n] s' →
-    φ' i s
-  | unlock : ∀ i i' s s',
-    φ' i' s' →
-    imp_step i [Method.unlock] i' →
-    spec_step s [Method.unlock] s' →
-    φ' i s
-  | lock : ∀ i i' s s',
-    φ' i' s' →
-    imp_step i [Method.lock] i' →
-    spec_step s [Method.lock] s' →
-    φ' i s
-  | internal : ∀ i i' s,
-    φ' i' s →
-    imp_step i [] i' →
-    φ' i s
-
+/-- 
+We define phi with a few necessary extensions.  For example, we use
+quantification for the `enq` case, so that we can handle any inputs and still
+commute.  In addition to that, we have indistinguishability inside of the φ.
+This is because
+-/
 inductive φ : ImpState → SpecState → Prop where
   | base :
     φ ⟨false, []⟩ ⟨[]⟩
@@ -150,85 +126,214 @@ theorem φ_length i s :
   | internal i i' s _ Hphi Himp Hlist =>
     cases Himp; assumption
 
+macro "solve_indistinguishable" t:tactic : tactic => 
+  `(tactic| (unfold indistinguishable; intros _ _ a; have Hindimpstep := a; cases a 
+             <;> (try ((repeat' first | (apply star.refl; done) | apply star.plus_one | constructor | $t:tactic) <;> done))))
+
+theorem invert_single_spec_step (s1 s2 : SpecState) (e : Method):
+  s1 -[[e]]*> s2 → s1 -[[e]]-> s2 := by
+  generalize Hthis : [e] = e'; intros Hs
+  cases Hs with
+  | refl => simp at Hthis
+  | step s1' s2' s3' e1 e2 Hstep Hstar =>
+    have Hthis' : e1 = [e] ∧ e2 = [] := by 
+      cases Hstep <;> (simp at *; tauto)
+    cases Hthis'; subst e1; subst e2
+    generalize Hother : [] = e' at Hstar
+    cases Hstar with 
+   | step s1'' s2'' s3'' e1' e2' Hstep' Hstar' =>
+      symm at Hother; rw [List.append_eq_nil] at Hother; cases Hother
+      subst e1'; subst e2'; cases Hstep'
+    | refl => assumption
+
+open Lean Elab Meta Tactic
+
+/--
+Tactic to specialize all the hypotheses in the context that contain an binding
+of that term in the first position.
+-/
+syntax (name := specializeAll) "specializeAll " term : tactic
+
+@[tactic specializeAll] def specializeAllTactic : Tactic
+  | `(tactic| specializeAll $t:term) => withMainContext do
+    let t ← elabTerm t none
+    let termType ← inferType t
+    let lctx ← getLCtx
+    lctx.forM fun decl : LocalDecl => do
+      -- First we check if the current hypothesis contains a binding of the same
+      -- type as the input term in the first position.
+      if (← forallTelescopeReducing decl.type fun vars _ => do
+        if h : vars.size > 0 then
+          isDefEq (← inferType vars[0]) termType
+        else
+          return false) 
+        -- We don't want to instantiate arrow types (only dependent types).
+        && decl.type.arrow?.isNone
+      then
+        let e ← mkAppM' decl.toExpr #[t]
+        -- We create a new assertion in the current goal and also infer the type
+        -- of `e` again.  Instead we could generate the correct type as well.
+        let mvarId ← (← getMainGoal).assert decl.userName (← inferType e).headBeta e
+        let (_, mvarId) ← mvarId.intro1P
+        let mvarId ← mvarId.tryClear decl.fvarId
+        replaceMainGoal [mvarId]
+      else
+        return ()
+  | _ => throwUnsupportedSyntax
+
+def kAbstractMatches (expr t : Expr) : MetaM Bool := do
+  try
+    -- `==` does not work here because sometimes the term can be reduced I
+    -- believe, in which case they won't 100% match.
+    let _ ← withAssignableSyntheticOpaque <| kabstract expr t
+    if not (← withAssignableSyntheticOpaque <| isDefEq (← kabstract expr t) expr) then
+      return true
+    else
+      return false
+  -- isDefEq will error with unbound bvars, which is expected and means
+  -- that the abstraction worked.
+  catch _e =>
+    return true
+
+def findIndHyp : TacticM (FVarId × FVarId) := do
+    -- First: Figure out which hypothesis is the top step and which is the
+    -- inductive hypothesis.  This will be made with the assumption that the
+    -- inductive hypothesis will contain the implementation step, implying a
+    -- series of specification steps and the phi.
+    let lctx ← getLCtx
+
+    -- log m!"{repr (∃ s', s -[ e ]*> s' ∧ φ i' s')}"
+
+    let mut ret := none
+
+    for decl in lctx do
+      -- Otherwise the theorem itself shows up in the declarations.
+      if decl.isImplementationDetail then continue
+
+      trace[debug] m!"(DECL) {decl.userName}: {decl.type}"
+
+      -- This will match different step functions, which can then be used to
+      -- find the inductive hypothesis.
+      let (x, ind_hyp') ← withNewMCtxDepth do
+        let (_, _, expr) ← forallMetaTelescopeReducing decl.type
+        let t ← elabTermWithHoles (← `(imp_step ?a ?b ?c)) none `createInductivePhi
+        let s ← elabTerm (← `(imp_step ?c ?d ?e)) none
+        -- trace[debug] m!"T':: {t.fst}"
+        -- trace[debug] m!"(DECL2): {expr}"
+        -- trace[debug] m!"(DECL3): {repr expr}"
+        trace[debug] m!"(MAGIC): {(← withAssignableSyntheticOpaque <| kabstract expr t.fst)}"
+        if ← kAbstractMatches expr t.fst then
+          let mut declId := false
+          let mut ind_hyp : Array FVarId := #[]
+          for decl' in lctx do
+            if decl'.isImplementationDetail then continue
+
+            -- Using `forallMetaTelescopeReducing` here is necessary because
+            -- otherwise a new context is created that is not a `subPrefixOf`
+            -- the previous context.  This means that meta variables cannot be
+            -- instantiated in that context.
+            let (lst, _, expr') ← forallMetaTelescopeReducing decl'.type
+            match ← whnf expr' with
+            | .app (.app (.const ``Exists _) _) _ =>
+              
+              trace[debug] m!"(LIST): {← sequence <| List.map (inferType ·) (lst.toList)}"
+              for hyp in lst do
+                trace[debug] m!"(MAGIC2): {(← withAssignableSyntheticOpaque <| kabstract (← inferType hyp) s)}"
+                if ← kAbstractMatches (← inferType hyp) s then
+                  declId := true
+                  ind_hyp := ind_hyp.push decl'.fvarId
+                trace[debug] m!"TYPE: {(← inferType hyp)} ::: {s}"
+                trace[debug] m!"DECLUSERNAME: {decl'.userName}: {← inferType hyp}"
+            | _ => pure ()
+          return (declId, ind_hyp)
+        else return (false, #[])
+      if h : x ∧ ind_hyp'.size > 0 then
+        ret := some (decl.fvarId, ind_hyp'[0])
+
+    let some someret := ret
+        | throwError "Could not find hypothesis"
+    return someret
+
+def findCurrentEvent : TacticM Expr := do
+  let (.app (.app (.const ``Exists _) _) goalType) := (← getMainTarget).consumeMData 
+    | throwError "Not the right goal type"
+  withNewMCtxDepth <| lambdaTelescope goalType fun _ars newGoalType => do
+    let (t, ars) ← elabTermWithHoles (← `(@star SpecState Method _ ?a ?b ?c)) none `findCurrentEvent
+    if ← kAbstractMatches newGoalType t then
+      instantiateMVars (Expr.mvar ars[1]!)
+    else throwError "Could not find event type in goal"
+
+/--
+Creates
+-/
+syntax (name := createInductivePhi) "create_ind_phi" : tactic
+
+@[tactic createInductivePhi] def createInductivePhiTactic : Tactic
+  | `(tactic| create_ind_phi) => withMainContext do
+    let lctx ← getLCtx
+    let (imp, ind) ← findIndHyp
+    trace[debug] m!"Found : {(lctx.get! imp).userName} and {(lctx.get! ind).userName}"
+    let e ← findCurrentEvent
+    trace[debug] m!"FOUND: {e}"
+    liftMetaTactic fun mvarId => do
+      let ind_decl := lctx.get! ind
+      let (ars, _, t) ← forallMetaTelescopeReducing ind_decl.type
+      for x in ars do
+        if ← isDefEq (← inferType x) (← inferType e) then
+          x.mvarId!.assign e
+      let e_t ← mkAppM' ind_decl.toExpr ars
+      let mvarIdNew ← mvarId.define ind_decl.userName t e_t
+      let (_, mvarIdNew) ← mvarIdNew.intro1P
+      sequence <| (mvarIdNew :: (ars.map (·.mvarId!)).toList.reverse).map (·.tryClear ind)
+  | _ => throwUnsupportedSyntax
+
+/--
+Implementation of have with holes, which uses let first to create the definition
+and then assigns it using `have` to remove the body, followed by clearing the
+hypothesis.
+-/
+syntax (name := haveByLet) "have_hole " haveDecl : tactic
+
+macro_rules
+  | `(tactic| have_hole $id:haveId $bs* : $type := $proof) => 
+    `(tactic| (let h $bs* : $type := $proof; have $id:haveId := h; clear h))
+set_option pp.all true
 theorem enough :
-  ∀ i s, φ i s →
+  ∀ i s, φ i s→ 
     ∀ e i', imp_step i e i' → 
       ∃ s', star s e s' ∧ φ i' s' := by
-  intros i s h;
+  intro i s h;
   induction h with
   | base =>
-    intros e i' Himp
+    intro e i' Himp
     cases Himp with
     | handle_enq n a =>
       simp; exists ⟨[n]⟩; and_intros
       · apply step_one; constructor
       · apply φ.deq
+        · solve_indistinguishable (simp [*] at *)
         · apply φ.base
         · constructor; simp; rfl
         · constructor; simp
-      · unfold indistinguishable at *
-        intros e i' Histep
-        cases Histep with
-        | handle_enq n' a' =>
-          simp at *
-          constructor; apply star.plus_one
-          constructor
-        | handle_deq n' rst' a' =>
-          simp at *
-          rcases a' with ⟨ Hl, Hr ⟩
-          constructor; apply star.plus_one
-          constructor; simp
-          and_intros <;> [congr; rfl]
-        | handle_lock | handle_unlock =>
-          constructor; apply star.plus_one; constructor
-        | unlock_natural => constructor; apply star.refl
     | handle_deq n rst a => simp at a
     | handle_lock =>
       simp; exists ⟨[]⟩; and_intros
       · apply star.plus_one; constructor
-      · apply φ.unlock; apply φ.base
+      · apply φ.unlock
+        · solve_indistinguishable (simp [*] at *)
+        · apply φ.base
         · constructor
         · constructor
-      · unfold indistinguishable at *
-        intros e i' Histep
-        cases Histep with
-        | handle_enq n' a' => simp at *
-        | handle_deq n' rst' a' => simp at *
-        | handle_lock | handle_unlock =>
-          constructor; apply star.plus_one; constructor
-        | unlock_natural => constructor; apply star.refl
     | handle_unlock =>
       simp; exists ⟨[]⟩; and_intros
       · apply star.plus_one; constructor
       · apply φ.base
-      · unfold indistinguishable at *
-        intros e i' Histep
-        cases Histep with
-        | handle_enq n' a' =>
-          simp at *
-          constructor; apply star.plus_one
-          constructor
-        | handle_deq n' rst' a' => simp at *
-        | handle_lock | handle_unlock =>
-          constructor; apply star.plus_one; constructor
-        | unlock_natural => constructor; apply star.refl
     | unlock_natural a =>
       simp; exists ⟨[]⟩; and_intros
       · apply star.refl
       · apply φ.base
-      · unfold indistinguishable at *
-        intros e i' Histep
-        cases Histep with
-        | handle_enq n' a' =>
-          simp at *
-          constructor; apply star.plus_one
-          constructor
-        | handle_deq n' rst' a' => simp at *
-        | handle_lock | handle_unlock =>
-          constructor; apply star.plus_one; constructor
-        | unlock_natural => constructor; apply star.refl
-  | enq i i_ne s s_ne i_wf s_wf Hphi HimpRight HspecRight iH =>
-    intros e i_sw HimpDown
+  | enq i i_ne s s_ne i_wf s_wf Hindist Hphi HimpRight HspecRight iH =>
+    intro e i_sw HimpDown
     have HimpDown' := HimpDown
     cases HimpDown with
     | handle_enq n' Hlock =>
@@ -237,25 +342,80 @@ theorem enough :
       and_intros
       · apply star.plus_one; constructor
       · assumption
-      · unfold indistinguishable at *
-        intros e' i' Histep
-        cases Histep with
-        | handle_enq n' a' => constructor; apply star.plus_one; constructor
-        | handle_deq n'' rst' a' =>
-          
     | handle_deq n' rst Hqueue =>
-      let Himp2' : ∀ n, imp_step (i_ne n) [Method.deq n'] _ := by
-        intros n''; rw [i_wf, Hqueue]; constructor; simp; rfl
-      have Himp2 := Himp2'; clear Himp2'
-      simp at *
-      let iH' : ∀ n, ∃ s', s_ne n -[ [Method.deq n'] ]*> s' ∧ φ { lock := i.lock, queue := rst ++ [n] } s' := by
-        intros n''; apply iH
-        apply Himp2
-      have iH'' := iH'; clear iH'
-      rcases s with ⟨ queue ⟩
-      rcases queue with _ | ⟨ a, b ⟩
-
-      constructor; and_intros
+      create_ind_phi; rotate_left
+      specializeAll ?n
+      apply imp_step.handle_deq
+      run_tac do
+        withAssignableSyntheticOpaque <| evalTactic (← `(tactic| apply imp_step.handle_deq))
       
+      rw [i_wf, Hqueue]; constructor; simp; rfl
+      have_hole Himp2 : ∀ n, imp_step (i_ne n) [Method.deq n'] _ := by
+        
+      simp at *
+      -- have_hole iH' : ∀ n, ∃ s', s_ne n -[ [Method.deq n'] ]*> s' ∧ φ { lock := i.lock, queue := rst ++ [n] } s' := by
+      --   intro n''; apply iH
+      --   apply Himp2
+      have HimpDown'' := HimpDown'
+      apply Hindist at HimpDown'
+      rcases HimpDown' with ⟨ s_sw, HspecDown' ⟩
+      exists s_sw; and_intros <;> try assumption
+      have_hole HimpDownR : ∀ n, imp_step (i_ne n) [Method.deq n'] _ := by
+        intro n
+        constructor
+        rw [i_wf]; simp; rw [Hqueue]; rfl
+      have hfinalphi: ∀ n, φ { lock := i.lock, queue := rst ++ [n] } { queue := s_sw.queue ++ [n] } := by
+        intro n
+        specializeAll n
+        --specializeAll 0
+        apply iH at HimpDownR
+        rcases HimpDownR with ⟨ s_se, HspecRightD, Hphi_se ⟩
+        rw [s_wf] at *; rw [i_wf] at *
+        clear i_wf; clear s_wf
+        simp at Hphi_se
+        apply invert_single_spec_step at HspecDown'
+        rcases HspecDown' with _ | ⟨ _, rst', Ha ⟩
+        apply invert_single_spec_step at HspecRightD
+        rcases HspecRightD with _ | ⟨ _, rst'', Ha' ⟩
+        simp only [*] at *
+        have : rst' ++ [n] = rst'' := by cases Ha'; dsimp
+        subst rst''; assumption
+      apply φ.enq
+      · intros; rfl
+      · intros; rfl
+      · solve_indistinguishable fail
+        specialize hfinalphi 0
+        apply φ_indistinguishable at hfinalphi
+        unfold indistinguishable at *
+        rename_i n rst' a Hindimpstep
+        have_hole : ({ lock := i.lock, queue := rst ++ [0] } : ImpState) -[ [Method.deq n] ]-> _ := by
+          constructor; simp only at a; rw [a]; rfl
+        apply hfinalphi at this
+        rcases this with ⟨ hns, H ⟩
+        apply invert_single_spec_step at H
+        rcases H with _ | ⟨ _, rst''', Ha'' ⟩ | _
+        simp at *
+        generalize Hgen : s_sw.queue = e at *
+        cases e
+        . simp at *; cases Ha''; subst n; subst rst'''
+          have : φ i s := φ.enq i i_ne s s_ne i_wf s_wf Hindist Hphi HimpRight HspecRight
+          apply φ_length at this
+          rcases HimpDown'' with _ | ⟨ _, _, c ⟩
+          subst rst
+          apply invert_single_spec_step at HspecDown'
+          cases HspecDown'; simp at *
+          rename_i rst'''' a''''
+          subst rst''''; rw [a''''] at this
+          rw [Hqueue] at this; simp at this
+        · simp at *; cases Ha''; subst n; subst rst'''
+          (repeat' first | apply star.plus_one | rw [← Hgen] | constructor)
+      · assumption
+      · intros; constructor; specialize HimpRight 0; 
+        generalize Hother : i_ne 0 = i' at *; cases HimpRight; simp [*]
+      . intros; constructor
+    | handle_lock => sorry
+    | handle_unlock => sorry
+    | unlock_natural => sorry
+  | _ => sorry
 
 end DataflowRewriter
